HOL_To_IMP_Minus/Refinements/HOL_To_IMP_Minus_Arithmetics.thy
@@ -1,0 +1,209 @@
+\<^marker>\<open>creator "Kevin Kappelmann"\<close>
+theory HOL_To_IMP_Minus_Arithmetics
+  imports
+    HOL_To_IMP_Minus_Primitives
+    "HOL-Library.Discrete"
+begin
+
+context HOL_To_IMP_Minus
+begin
+
+definition [compiled_const_defs add]: "suc_IMP \<equiv> Com.Assign ''suc_ret'' (V ''suc_x'' \<oplus> N 1)"
+
+declare_compiled_const Suc
+  return_register "suc_ret"
+  argument_registers "suc_x"
+  compiled suc_IMP
+
+lemma suc_IMP_func_correct [func_correct]:
+  assumes "(suc_IMP, s) \<Rightarrow>\<^bsup>t\<^esup> s'"
+  shows "s' ''suc_ret'' = Suc (s ''suc_x'')"
+  using assms unfolding suc_IMP_def by auto
+
+fun mul_acc_nat :: "nat \<Rightarrow> nat \<Rightarrow> nat \<Rightarrow> nat" where
+  "mul_acc_nat x y z = (if x \<noteq> 0 then mul_acc_nat (x - 1) y (z + y) else z)"
+declare mul_acc_nat.simps[simp del]
+
+compile_nat mul_acc_nat.simps basename mul_acc
+
+lemma mul_acc_nat_IMP_func_correct[func_correct]:
+  assumes "(tailcall_to_IMP_Minus mul_acc_IMP, s) \<Rightarrow>\<^bsup>t\<^esup> s'"
+  shows "s' ''mul_acc_ret'' = mul_acc_nat (s ''mul_acc_x'') (s ''mul_acc_y'') (s ''mul_acc_z'')"
+  using assms                                 
+  apply (rule tailcall_to_IMP_Minus_correct_if_correct)
+  apply (simp add: mul_acc_IMP_def)
+  apply (simp add: mul_acc_IMP_def)
+  subgoal for t s'
+  apply (induction "(s ''mul_acc_x'')" "(s ''mul_acc_y'')" "(s ''mul_acc_z'')" arbitrary: s t rule: mul_acc_nat.induct)
+  apply (tactic \<open>H.run_finish_tac @{thms mul_acc_nat.simps} @{thm mul_acc_IMP_def}
+    @{thms func_correct} @{context} 1\<close>)
+  done
+  done
+
+lemma mul_acc_nat_eq_mul_add[simp]: "mul_acc_nat x y z = x * y + z"
+  by (induction x y z arbitrary: z rule: mul_acc_nat.induct)
+  (auto simp: mul_acc_nat.simps mult_eq_if)
+  
+definition mul_nat :: "nat \<Rightarrow> nat \<Rightarrow> nat" where
+  "mul_nat x y = mul_acc_nat x y 0"
+  
+compile_nat mul_nat_def basename mul
+
+declare_compiled_const "times"
+  return_register "mul_ret"
+  argument_registers "mul_x" "mul_y"
+  compiled "tailcall_to_IMP_Minus mul_IMP"
+
+lemma mul_nat_IMP_func_correct[func_correct]:
+  assumes "(tailcall_to_IMP_Minus mul_IMP, s) \<Rightarrow>\<^bsup>t\<^esup> s'"
+  shows "s' ''mul_ret'' = mul_nat (s ''mul_x'') (s ''mul_y'')"
+  using assms                                 
+  apply (rule tailcall_to_IMP_Minus_correct_if_correct)
+  apply (simp add: mul_IMP_def)
+  apply (simp add: mul_IMP_def)
+  apply (tactic \<open>H.run_finish_tac @{thms mul_nat_def} @{thm mul_IMP_def}
+    @{thms func_correct} @{context} 1\<close>)
+  done
+
+lemma mul_nat_eq_mul[simp]: "mul_nat x y = x * y"
+  unfolding mul_nat_def by simp
+
+fun div_acc_nat :: "nat \<Rightarrow> nat \<Rightarrow> nat \<Rightarrow> nat" where
+  "div_acc_nat x y z = (if y = 0 then z else if x < y then z else div_acc_nat (x - y) y (z + 1))"
+declare div_acc_nat.simps[simp del]
+
+compile_nat div_acc_nat.simps basename div_acc
+
+lemma div_acc_nat_IMP_func_correct[func_correct]:
+  assumes "(tailcall_to_IMP_Minus div_acc_IMP, s) \<Rightarrow>\<^bsup>t\<^esup> s'"
+  shows "s' ''div_acc_ret'' = div_acc_nat (s ''div_acc_x'') (s ''div_acc_y'') (s ''div_acc_z'')"
+  using assms                                 
+  apply (rule tailcall_to_IMP_Minus_correct_if_correct)
+  apply (simp add: div_acc_IMP_def)
+  apply (simp add: div_acc_IMP_def)
+  subgoal for t s'
+  apply (induction "(s ''div_acc_x'')" "(s ''div_acc_y'')" "(s ''div_acc_z'')" arbitrary: s t rule: div_acc_nat.induct)
+  apply (tactic \<open>H.run_finish_tac @{thms div_acc_nat.simps} @{thm div_acc_IMP_def}
+    @{thms func_correct} @{context} 1\<close>)
+  done
+  done
+
+lemma div_acc_nat_eq_div[simp]: "div_acc_nat x y z = x div y + z"
+  by (induction x y z rule: div_acc_nat.induct) (auto simp: div_acc_nat.simps div_if)
+
+definition div_nat :: "nat \<Rightarrow> nat \<Rightarrow> nat" where
+  "div_nat x y = div_acc_nat x y 0"
+
+compile_nat div_nat_def basename div
+
+declare_compiled_const "divide"
+  return_register "div_ret"
+  argument_registers "div_x" "div_y"
+  compiled "tailcall_to_IMP_Minus div_IMP"
+
+lemma div_nat_IMP_func_correct[func_correct]:
+  assumes "(tailcall_to_IMP_Minus div_IMP, s) \<Rightarrow>\<^bsup>t\<^esup> s'"
+  shows "s' ''div_ret'' = div_nat (s ''div_x'') (s ''div_y'')"
+  using assms                                 
+  apply (rule tailcall_to_IMP_Minus_correct_if_correct)
+  apply (simp add: div_IMP_def)
+  apply (simp add: div_IMP_def)
+  apply (tactic \<open>H.run_finish_tac @{thms div_nat_def} @{thm div_IMP_def}
+    @{thms func_correct} @{context} 1\<close>)
+  done
+
+lemma div_nat_eq_div[simp]: "div_nat x y = x div y"
+  unfolding div_nat_def by simp
+
+definition square_nat :: "nat \<Rightarrow> nat" where
+  "square_nat x \<equiv> mul_nat x x"
+  
+compile_nat square_nat_def basename square
+
+lemma square_nat_IMP_func_correct[func_correct]:
+  assumes "(tailcall_to_IMP_Minus square_IMP, s) \<Rightarrow>\<^bsup>t\<^esup> s'"
+  shows "s' ''square_ret'' = square_nat (s ''square_x'')"
+  using assms                                 
+  apply (rule tailcall_to_IMP_Minus_correct_if_correct)
+  apply (simp add: square_IMP_def)
+  apply (simp add: square_IMP_def)
+  apply (tactic \<open>H.run_finish_tac @{thms square_nat_def} @{thm square_IMP_def}
+    @{thms func_correct} @{context} 1\<close>)
+  done
+
+lemma square_nat_eq_square[simp]: "square_nat x = x\<^sup>2"
+  unfolding square_nat_def by (simp add: power2_eq_square)
+
+(*takes lower and upper bound for root*)
+function sqrt_aux_nat :: "nat \<Rightarrow> nat \<Rightarrow> nat \<Rightarrow> nat" where
+  "sqrt_aux_nat x L R = (if Suc L < R
+    then 
+      let M = (L + R) div 2
+      in 
+        if square_nat M \<le> x
+        then sqrt_aux_nat x M R 
+        else sqrt_aux_nat x L M 
+    else L)"
+  by auto
+termination by (relation "Wellfounded.measure (\<lambda>(_, L, R). R - L)") auto
+declare sqrt_aux_nat.simps[simp del]
+
+compile_nat sqrt_aux_nat.simps basename sqrt_aux
+
+lemma sqrt_aux_IMP_func_correct[func_correct]:
+  assumes "(tailcall_to_IMP_Minus sqrt_aux_IMP, s) \<Rightarrow>\<^bsup>t\<^esup> s'"
+  shows "s' ''sqrt_aux_ret'' = sqrt_aux_nat (s ''sqrt_aux_x'') (s ''sqrt_aux_L'') (s ''sqrt_aux_R'')"
+  using assms                                 
+  apply (rule tailcall_to_IMP_Minus_correct_if_correct)
+  apply (subst compiled_const_defs, simp)
+  apply (subst compiled_const_defs, simp)
+  subgoal for t s'
+  apply (induction "s ''sqrt_aux_x''" "s ''sqrt_aux_L''" "s ''sqrt_aux_R''" arbitrary: s t rule: sqrt_aux_nat.induct)
+  apply (tactic \<open>H.run_finish_tac @{thms sqrt_aux_nat.simps} @{thm sqrt_aux_IMP_def}
+    @{thms func_correct} @{context} 1\<close>)
+  done
+  done
+
+lemma square_sqrt_aux_nat_le:
+  assumes "L\<^sup>2 \<le> x" "x < R\<^sup>2"
+  shows "(sqrt_aux_nat x L R)\<^sup>2 \<le> x"
+  using assms
+  by (induction x L R rule: sqrt_aux_nat.induct)
+  (auto simp: sqrt_aux_nat.simps Let_def)
+  
+lemma lt_square_Suc_sqrt_aux_nat:
+  assumes "L\<^sup>2 \<le> x" "x < R\<^sup>2"
+  shows "x < (Suc (sqrt_aux_nat x L R))\<^sup>2"
+  using assms
+  by (induction x L R rule: sqrt_aux_nat.induct)
+  (use order_less_le_trans in \<open>force simp: sqrt_aux_nat.simps Let_def\<close>)
+
+definition sqrt_nat :: "nat \<Rightarrow> nat" where
+  "sqrt_nat x = sqrt_aux_nat x 0 (Suc x)"
+
+compile_nat sqrt_nat_def basename sqrt
+
+lemma sqrt_IMP_func_correct[func_correct]:
+  assumes "(tailcall_to_IMP_Minus sqrt_IMP, s) \<Rightarrow>\<^bsup>t\<^esup> s'"
+  shows "s' ''sqrt_ret'' = sqrt_nat (s ''sqrt_x'')"
+  using assms                                 
+  apply (rule tailcall_to_IMP_Minus_correct_if_correct)
+  apply (subst compiled_const_defs, simp)
+  apply (subst compiled_const_defs, simp)
+  apply (tactic \<open>H.run_finish_tac @{thms sqrt_nat_def} @{thm sqrt_IMP_def}
+    @{thms func_correct} @{context} 1\<close>)
+  done
+
+lemma square_sqrt_nat_le: "(sqrt_nat x)\<^sup>2 \<le> x"
+  using square_sqrt_aux_nat_le unfolding sqrt_nat_def by (simp add: power2_eq_square)
+
+lemma lt_square_Suc_sqrt_nat: "x < (Suc (sqrt_nat x))\<^sup>2"
+  using lt_square_Suc_sqrt_aux_nat unfolding sqrt_nat_def by (simp add: power2_eq_square)
+
+corollary sqrt_nat_sqrt[simp]: "sqrt_nat y = Discrete.sqrt y"
+  using square_sqrt_nat_le lt_square_Suc_sqrt_nat
+  by (intro sqrt_unique[symmetric]) auto
+
+end
+
+end
