HOL_To_IMP_Minus/Refinements/HOL_To_IMP_Minus_Datatypes.thy
@@ -1,0 +1,28 @@
+\<^marker>\<open>creator "Kevin Kappelmann"\<close>
+theory HOL_To_IMP_Minus_Datatypes
+  imports
+    HOL_To_IMP_Minus_Arithmetics
+    "HOL-Library.Nat_Bijection"
+begin
+
+context HOL_To_IMP_Minus
+begin
+
+compile_nat triangle_def basename triangle
+
+lemma triangle_IMP_func_correct [func_correct]:
+  assumes "(tailcall_to_IMP_Minus triangle_IMP, s) \<Rightarrow>\<^bsup>t\<^esup> s'"
+  shows "s' ''triangle_ret'' = triangle (s ''triangle_n'')"
+  using assms
+  apply (rule tailcall_to_IMP_Minus_correct_if_correct)
+  apply (subst compiled_const_defs, simp)
+  apply (subst compiled_const_defs, simp)
+  apply (tactic \<open>H.run_finish_tac @{thms triangle_def} @{thm triangle_IMP_def}
+    @{thms func_correct} @{context} 1\<close>)
+  done
+
+text \<open>up next: encoding of products, sums, etc. See @{term prod_encode}\<close>
+
+end
+
+end
