HOL_To_IMP_Minus/Refinements/HOL_To_IMP_Minus_Primitives.thy
@@ -1,0 +1,305 @@
+\<^marker>\<open>creator "Kevin Kappelmann"\<close>
+theory HOL_To_IMP_Minus_Primitives
+  imports
+    HOL_To_IMP_Tailcalls_Tactics
+begin
+
+locale HOL_To_IMP_Minus =
+  notes neq0_conv[iff del, symmetric, iff]
+begin
+
+named_theorems func_correct
+
+definition "is_true_nat n \<equiv> n \<noteq> 0"
+
+lemma is_true_nat_eq[simp]: "is_true_nat = (\<noteq>) 0"
+  unfolding is_true_nat_def by simp
+
+definition "is_false_nat n \<equiv> n = 0"
+
+lemma is_false_nat_iff[iff]: "is_false_nat n \<longleftrightarrow> \<not>(is_true_nat n)"
+  unfolding is_false_nat_def by simp
+
+definition "true_nat \<equiv> (1 :: nat)"
+
+compile_nat true_nat_def basename true
+
+declare_compiled_const True
+  return_register "true_ret"
+  argument_registers
+  compiled "tailcall_to_IMP_Minus true_IMP"
+
+lemma true_IMP_func_correct[func_correct]:
+  assumes "(tailcall_to_IMP_Minus true_IMP, s) \<Rightarrow>\<^bsup>t\<^esup> s'"
+  shows "s' ''true_ret'' = true_nat"
+  using assms
+  apply (rule tailcall_to_IMP_Minus_correct_if_correct)
+  apply (subst compiled_const_defs, simp)
+  apply (subst compiled_const_defs, simp)
+  apply (tactic \<open>H.run_finish_tac @{thms true_nat_def} @{thm true_IMP_def}
+    @{thms func_correct} @{context} 1\<close>)
+  done
+
+lemma true_nat_eq_one[simp]: "true_nat = 1"
+  unfolding true_nat_def by simp
+
+lemma is_true_nat_true_nat[iff]: "is_true_nat true_nat"
+  by simp
+
+definition "false_nat \<equiv> 0"
+
+compile_nat false_nat_def basename false
+
+declare_compiled_const False
+  return_register "false_ret"
+  argument_registers
+  compiled "tailcall_to_IMP_Minus false_IMP"
+
+lemma false_IMP_func_correct [func_correct]:
+  assumes "(tailcall_to_IMP_Minus false_IMP, s) \<Rightarrow>\<^bsup>t\<^esup> s'"
+  shows "s' ''false_ret'' = false_nat"
+  using assms
+  apply (rule tailcall_to_IMP_Minus_correct_if_correct)
+  apply (subst compiled_const_defs, simp)
+  apply (subst compiled_const_defs, simp)
+  apply (tactic \<open>H.run_finish_tac @{thms false_nat_def} @{thm false_IMP_def}
+    @{thms func_correct} @{context} 1\<close>)
+  done
+
+lemma false_nat_eq_one[simp]: "false_nat = 0"
+  unfolding false_nat_def by simp
+
+lemma is_false_nat_false_nat[iff]: "is_false_nat false_nat"
+  unfolding false_nat_def by simp
+
+definition "id_nat x \<equiv> x"
+
+compile_nat id_nat_def basename id
+
+lemma id_IMP_func_correct [func_correct]:
+  assumes "(tailcall_to_IMP_Minus id_IMP, s) \<Rightarrow>\<^bsup>t\<^esup> s'"
+  shows "s' ''id_ret'' = id_nat (s ''id_x'')"
+  using assms
+  apply (rule tailcall_to_IMP_Minus_correct_if_correct)
+  apply (subst compiled_const_defs, simp)
+  apply (subst compiled_const_defs, simp)
+  apply (tactic \<open>H.run_finish_tac @{thms id_nat_def} @{thm id_IMP_def}
+    @{thms func_correct} @{context} 1\<close>)
+  done
+
+lemma id_nat_eq_id[simp]: "id_nat = id"
+  unfolding id_nat_def by (rule ext) simp
+
+definition "nat_of_bool b \<equiv> if b then true_nat else false_nat"
+
+declare_compiled_const nat_of_bool
+  return_register "id_ret"
+  argument_registers "id_x"
+  compiled "tailcall_to_IMP_Minus id_IMP"
+
+lemma nat_of_bool_eq_zero_iff[iff]: "nat_of_bool b = 0 \<longleftrightarrow> \<not>b"
+  unfolding nat_of_bool_def by simp
+
+lemma nat_of_bool_neq_zero_iff[iff]: "nat_of_bool b \<noteq> 0 \<longleftrightarrow> b"
+  unfolding nat_of_bool_def by simp
+
+definition "eq_nat (n :: nat) m \<equiv> nat_of_bool (n = m)"
+
+context includes com_syntax no_com'_syntax
+begin
+
+definition [compiled_const_defs add]:
+  "eq_IMP \<equiv>
+    ''eq_x_Sub_y'' ::= (V ''eq_x'' \<ominus> V ''eq_y'');;
+    ''eq_y_Sub_x'' ::= (V ''eq_y'' \<ominus> V ''eq_x'');;
+    ''eq_neq'' ::= (V ''eq_x_Sub_y'' \<oplus> V ''eq_y_Sub_x'');;
+    IF ''eq_neq'' \<noteq>0
+    THEN ''eq_ret'' ::= A (N false_nat)
+    ELSE ''eq_ret'' ::= A (N true_nat)"
+
+end
+
+declare_compiled_const eq_nat
+  return_register "eq_ret"
+  argument_registers "eq_x" "eq_y"
+  compiled eq_IMP
+
+declare_compiled_const HOL.eq
+  return_register "eq_ret"
+  argument_registers "eq_x" "eq_y"
+  compiled eq_IMP
+
+lemma eq_IMP_func_correct [func_correct]:
+  assumes "(eq_IMP, s) \<Rightarrow>\<^bsup>t\<^esup> s'"
+  shows "s' ''eq_ret'' = eq_nat (s ''eq_x'') (s ''eq_y'')"
+  using assms unfolding eq_IMP_def eq_nat_def nat_of_bool_def by auto
+
+lemma eq_nat_eq_nat_of_bool_eq[simp]: "eq_nat n m = nat_of_bool (n = m)"
+  unfolding eq_nat_def by simp
+
+definition "not_nat (n :: nat) \<equiv> nat_of_bool (n = false_nat)"
+
+compile_nat not_nat_def basename not
+
+declare_compiled_const HOL.Not
+  return_register "not_ret"
+  argument_registers "not_n"
+  compiled "tailcall_to_IMP_Minus not_IMP"
+
+lemma not_IMP_func_correct [func_correct]:
+  assumes "(tailcall_to_IMP_Minus not_IMP, s) \<Rightarrow>\<^bsup>t\<^esup> s'"
+  shows "s' ''not_ret'' = not_nat (s ''not_n'')"
+  using assms                                 
+  apply (rule tailcall_to_IMP_Minus_correct_if_correct)
+  apply (simp add: not_IMP_def)
+  apply (simp add: not_IMP_def)
+  apply (tactic \<open>H.run_finish_tac @{thms not_nat_def} @{thm not_IMP_def}
+    @{thms func_correct} @{context} 1\<close>)
+  done
+
+lemma not_nat_eq_nat_of_bool_eq_false[simp]: "not_nat n = nat_of_bool (n = false_nat)"
+  unfolding not_nat_def by simp
+
+definition max_nat :: "nat \<Rightarrow> nat \<Rightarrow> nat" where
+  "max_nat x y \<equiv> if x - y \<noteq> 0 then x else y"  
+
+compile_nat max_nat_def basename max
+
+declare_compiled_const max
+  return_register "max_ret"
+  argument_registers "max_x" "max_y"
+  compiled "tailcall_to_IMP_Minus max_IMP"
+
+lemma max_IMP_func_correct[func_correct]:
+  assumes "(tailcall_to_IMP_Minus max_IMP, s) \<Rightarrow>\<^bsup>t\<^esup> s'"
+  shows "s' ''max_ret'' = max_nat (s ''max_x'') (s ''max_y'')"
+  using assms                                 
+  apply (rule tailcall_to_IMP_Minus_correct_if_correct)
+  apply (simp add: max_IMP_def)
+  apply (simp add: max_IMP_def)
+  apply (tactic \<open>H.run_finish_tac @{thms max_nat_def} @{thm max_IMP_def}
+    @{thms func_correct} @{context} 1\<close>)
+  done
+
+lemma max_nat_eq[simp]: "max_nat x y = max x y"
+  unfolding max_nat_def by simp
+
+definition min_nat :: "nat \<Rightarrow> nat \<Rightarrow> nat" where
+  "min_nat x y \<equiv> if x - y \<noteq> 0 then y else x"
+
+compile_nat min_nat_def basename min
+
+declare_compiled_const min
+  return_register "min_ret"
+  argument_registers "min_x" "min_y"
+  compiled "tailcall_to_IMP_Minus min_IMP"
+
+lemma min_IMP_func_correct[func_correct]:
+  assumes "(tailcall_to_IMP_Minus min_IMP, s) \<Rightarrow>\<^bsup>t\<^esup> s'"
+  shows "s' ''min_ret'' = min_nat (s ''min_x'') (s ''min_y'')"
+  using assms                                 
+  apply (rule tailcall_to_IMP_Minus_correct_if_correct)
+  apply (simp add: min_IMP_def)
+  apply (simp add: min_IMP_def)
+  apply (tactic \<open>H.run_finish_tac @{thms min_nat_def} @{thm min_IMP_def}
+    @{thms func_correct} @{context} 1\<close>)
+  done
+
+lemma min_nat_eq[simp]: "min_nat x y = min x y"
+  unfolding min_nat_def by simp
+
+definition "and_nat (x :: nat) y \<equiv> min (min x y) true_nat"
+  
+compile_nat and_nat_def basename "and"
+
+declare_compiled_const conj
+  return_register "and_ret"
+  argument_registers "and_x" "and_y"
+  compiled "tailcall_to_IMP_Minus and_IMP"
+
+lemma and_nat_IMP_func_correct[func_correct]:
+  assumes "(tailcall_to_IMP_Minus and_IMP, s) \<Rightarrow>\<^bsup>t\<^esup> s'"
+  shows "s' ''and_ret'' = and_nat (s ''and_x'') (s ''and_y'')"
+  using assms                                 
+  apply (rule tailcall_to_IMP_Minus_correct_if_correct)
+  apply (subst compiled_const_defs, simp)
+  apply (subst compiled_const_defs, simp)
+  apply (tactic \<open>H.run_finish_tac @{thms and_nat_def} @{thm and_IMP_def}
+    @{thms func_correct} @{context} 1\<close>)
+  done
+
+lemma and_nat_eq[simp]: "and_nat x y = nat_of_bool (is_true_nat x \<and> is_true_nat y)"
+  unfolding and_nat_def nat_of_bool_def by auto
+
+definition "or_nat (x :: nat) y \<equiv> min (max x y) true_nat"
+
+compile_nat or_nat_def basename "or"
+
+declare_compiled_const disj
+  return_register "or_ret"
+  argument_registers "or_x" "or_y"
+  compiled "tailcall_to_IMP_Minus or_IMP"
+
+lemma or_nat_IMP_func_correct[func_correct]:
+  assumes "(tailcall_to_IMP_Minus or_IMP, s) \<Rightarrow>\<^bsup>t\<^esup> s'"
+  shows "s' ''or_ret'' = or_nat (s ''or_x'') (s ''or_y'')"
+  using assms                                 
+  apply (rule tailcall_to_IMP_Minus_correct_if_correct)
+  apply (subst compiled_const_defs, simp)
+  apply (subst compiled_const_defs, simp)
+  apply (tactic \<open>H.run_finish_tac @{thms or_nat_def} @{thm or_IMP_def}
+    @{thms func_correct} @{context} 1\<close>)
+  done
+
+lemma or_nat_eq[simp]: "or_nat x y = nat_of_bool (is_true_nat x \<or> is_true_nat y)"
+  unfolding or_nat_def nat_of_bool_def by auto
+
+definition "le_nat (x :: nat) y \<equiv> nat_of_bool (x - y = 0)"
+
+compile_nat le_nat_def basename le
+
+declare_compiled_const "ord_class.less_eq"
+  return_register "le_ret"
+  argument_registers "le_x" "le_y"
+  compiled "tailcall_to_IMP_Minus le_IMP"
+
+lemma le_nat_IMP_func_correct[func_correct]:
+  assumes "(tailcall_to_IMP_Minus le_IMP, s) \<Rightarrow>\<^bsup>t\<^esup> s'"
+  shows "s' ''le_ret'' = le_nat (s ''le_x'') (s ''le_y'')"
+  using assms                                 
+  apply (rule tailcall_to_IMP_Minus_correct_if_correct)
+  apply (subst compiled_const_defs, simp)
+  apply (subst compiled_const_defs, simp)
+  apply (tactic \<open>H.run_finish_tac @{thms le_nat_def} @{thm le_IMP_def}
+    @{thms func_correct} @{context} 1\<close>)
+  done
+
+lemma le_nat_eq[simp]: "le_nat x y = nat_of_bool (x \<le> y)"
+  unfolding le_nat_def by simp
+
+definition "lt_nat (x :: nat) y \<equiv> nat_of_bool (x \<le> y \<and> x \<noteq> y)"
+
+compile_nat lt_nat_def basename lt
+
+declare_compiled_const "ord_class.less"
+  return_register "lt_ret"
+  argument_registers "lt_x" "lt_y"
+  compiled "tailcall_to_IMP_Minus lt_IMP"
+
+lemma lt_nat_IMP_func_correct[func_correct]:
+  assumes "(tailcall_to_IMP_Minus lt_IMP, s) \<Rightarrow>\<^bsup>t\<^esup> s'"
+  shows "s' ''lt_ret'' = lt_nat (s ''lt_x'') (s ''lt_y'')"
+  using assms                                 
+  apply (rule tailcall_to_IMP_Minus_correct_if_correct)
+  apply (subst compiled_const_defs, simp)
+  apply (subst compiled_const_defs, simp)
+  apply (tactic \<open>H.run_finish_tac @{thms lt_nat_def}  @{thm lt_IMP_def}
+    @{thms func_correct} @{context} 1\<close>)
+  done
+
+lemma lt_nat_eq[simp]: "lt_nat x y = nat_of_bool (x < y)"
+  unfolding lt_nat_def nat_of_bool_def by auto
+
+end
+
+end
