HOL_To_IMP_Minus/Views/IMP_Tailcalls/HOL_To_IMP_Tailcalls_Tactics.thy
@@ -1,0 +1,101 @@
+\<^marker>\<open>creator "Kevin Kappelmann"\<close>
+theory HOL_To_IMP_Tailcalls_Tactics
+  imports
+    States_IMP_Tailcalls
+    Compile_Nat
+    (*"HOL-Library.Simps_Case_Conv"*)
+begin
+
+lemma tailcall_to_IMP_Minus_complete:
+  assumes "(tailcall_to_IMP_Minus c, s) \<Rightarrow>\<^bsup>t\<^esup> s'"
+  and "invar c"
+  obtains t' s'' where
+    "c \<turnstile> (c, s) \<Rightarrow>\<^bsup>t' - 7\<^esup> s''" "s' = s'' on set (vars c)"
+    "t' \<le> t" "t \<le> (t' + 1) * (1 + size\<^sub>c (compile c))"
+proof -
+  from assms inline obtain t' s'' where
+    "(compile c, s) \<Rightarrow>'\<^bsup>t'\<^esup> s''"
+    "s' = s'' on set (vars (compile c))" and
+    t': "t' \<le> t" "t \<le> (t' + 1) * (1 + size\<^sub>c (compile c))"
+    unfolding tailcall_to_IMP_Minus_eq by blast
+  from compile_complete[OF this(1) \<open>invar c\<close>] obtain s''' where
+    "c \<turnstile> (c, s) \<Rightarrow>\<^bsup>t' - 7\<^esup> s'''" "s'' = s''' on set (vars c)"
+    by blast
+  with \<open>s' = s'' on set (vars (compile c))\<close> have "s' = s''' on set (vars c)"
+    by (simp add: eq_on_def set_vars_compile)
+  with \<open>c \<turnstile> (c, s) \<Rightarrow>\<^bsup>t' - 7\<^esup> s'''\<close> t' show ?thesis
+    using that by blast
+qed
+
+lemma tailcall_to_IMP_Minus_correct_if_correct:
+  assumes "(tailcall_to_IMP_Minus c, s) \<Rightarrow>\<^bsup>t\<^esup> s'"
+  and "invar c"
+  and "x \<in> set (vars c)"
+  and "\<And>t s'. c \<turnstile> (c, s) \<Rightarrow>\<^bsup>t\<^esup> s' \<Longrightarrow> s' x = v"
+  shows "s' x = v"
+proof -
+  from tailcall_to_IMP_Minus_complete[OF assms(1,2)] obtain t' s'' where
+    c_eval: "c \<turnstile> (c, s) \<Rightarrow>\<^bsup>t' - 7\<^esup> s''" and "s' = s'' on set (vars c)" by blast
+  with assms(3) have "s' x = s'' x" by blast
+  also from c_eval assms(4) have "... = v" by auto
+  finally show ?thesis .
+qed
+
+context includes Com.no_com_syntax IMP_Tailcalls_Dynamic.tcom_syntax
+begin
+
+lemma tAssignD: "c \<turnstile> (x ::= a, s) \<Rightarrow>\<^bsup>t\<^esup> s' \<Longrightarrow> t = 2 \<and> s' = s(x := aval a s)"
+  by auto
+
+theorem tIf_tE':
+  assumes "c \<turnstile>(IF b\<noteq>0 THEN c1 ELSE c2, s) \<Rightarrow>\<^bsup>t\<^esup>  s'"
+  obtains t' where "t = Suc t'" and "s b \<noteq> 0" and "c \<turnstile>(c1, s) \<Rightarrow>\<^bsup>t'\<^esup> s'"
+    | t' where "t = Suc t'" and "s b = 0" and "c \<turnstile>(c2, s) \<Rightarrow>\<^bsup>t'\<^esup> s'"
+  using assms by auto
+
+ML_file \<open>hol_to_imp_tailcalls_tactics.ML\<close>
+
+ML \<open>
+  structure H = HOL_To_IMP_Tailcalls_Tactics
+  structure SIT = State_IMP_Tailcalls
+\<close>
+
+(*lemma case_nat_eq_if: "(case n of 0 \<Rightarrow> x | Suc x \<Rightarrow> f x) = (if n = 0 then x else f (n - 1))"
+  unfolding Nitpick.case_nat_unfold by simp
+
+fun add_nat_pat :: "nat \<Rightarrow> nat \<Rightarrow> nat \<Rightarrow> nat" where
+"add_nat_pat 0 0 z = z" |
+"add_nat_pat 0 (Suc y) z = add_nat_pat 0 y (Suc z)" |
+"add_nat_pat (Suc x) y z = add_nat_pat x y (Suc z)"
+declare add_nat_pat.simps[simp del]
+                        
+case_of_simps add_nat_pat_eq[simplified Nitpick.case_nat_unfold] : add_nat_pat.simps
+compile_nat add_nat_pat_eq basename add_pat
+
+lemma add_nat_pat_IMP_func_correct[cl_func_correct]:
+  assumes "(inline (compile (add_pat_IMP)), s) \<Rightarrow>\<^bsup>t\<^esup> s'"
+  shows "s' ''add_pat_ret'' = add_nat_pat (s ''add_pat_x1a'') (s ''add_pat_x2a'') (s ''add_pat_x3ba'')"
+  using assms                                 
+  apply (rule inline_compile_correct_if_correct)
+  apply (simp add: add_pat_IMP_def)
+  apply (simp add: add_pat_IMP_def)
+  subgoal for t s'
+  apply (induction "(s ''add_pat_x1a'')" "(s ''add_pat_x2a'')" "(s ''add_pat_x3ba'')" arbitrary: s t rule: add_nat_pat.induct)
+  apply simp
+  apply (tactic \<open>H.run_finish_tac @{thms add_nat_pat.simps} @{thm add_pat_IMP_def} 
+    @{thms cl_func_correct} @{context} 1\<close>)
+  apply simp
+  apply (tactic \<open>H.run_tac @{thm add_pat_IMP_def} @{thms cl_func_correct} @{context} 1\<close>)
+  (*apply (tactic \<open>H.finish_non_tailcall_tac @{thms add_nat_pat.simps} @{context} 1\<close>)*)
+  apply (tactic \<open>SIT.rewrite_all_state_app_tac' (fn ctxt => View_Util.subst_first_tac ctxt o single) @{context} 1\<close>)
+  apply (tactic \<open>SIT.remove_state_eq_tac @{context} 1\<close>)
+  (*apply (tactic \<open>View_Util.subst_first_tac @{context} @{thms add_nat_pat.simps} 1\<close>)*)
+    (*THEN' VU.subst_first_tac ctxt HOL_program_eqs*)
+    (*THEN' TU.TRY' (REPEAT_ALL_NEW (VU.subst_first_tac ctxt @{thm Let_def} ORELSE' if_split_tac ctxt))*)
+    (*THEN_ALL_NEW finish_goal_tac)*)
+  oops
+*)
+end
+  
+
+end
