HOL_To_IMP_Minus/Views/View_Utils.thy
@@ -1,11 +1,12 @@
 \<^marker>\<open>creator "Kevin Kappelmann"\<close>
 theory View_Utils
   imports
+    ML_Unification.ML_Tactic_Utils
     HOL.HOL
 begin
 
 paragraph \<open>Summary\<close>
-text \<open>Shared Utilities for @{session IMP_Minus_Views}.\<close>
+text \<open>General ML utilities to track IMP state changes.\<close>
 
 ML_file\<open>util.ML\<close>
 
